DynamoDbEncryption/dafny/DynamoDbEncryption/src/AwsCryptographyDbEncryptionSdkDynamoDbOperations.dfy
@@ -5,6 +5,12 @@ include "DynamoDbEncryptionBranchKeyIdSupplier.dfy"
 
 module AwsCryptographyDbEncryptionSdkDynamoDbOperations refines AbstractAwsCryptographyDbEncryptionSdkDynamoDbOperations {
   import DynamoDbEncryptionBranchKeyIdSupplier
+  import EdkWrapping
+  import UUID
+  import AlgorithmSuites
+  import DynamoToStruct
+
+  import Header = StructuredEncryptionHeader
 
   predicate ValidInternalConfig?(config: InternalConfig)
   {true}
@@ -32,5 +38,77 @@ module AwsCryptographyDbEncryptionSdkDynamoDbOperations refines AbstractAwsCrypt
           branchKeyIdSupplier := supplier
         )
     );
+  }
+  predicate GetEncryptedDataKeyDescriptionEnsuresPublicly(input: GetEncryptedDataKeyDescriptionInput , output: Result<GetEncryptedDataKeyDescriptionOutput, Error>)
+  {true}
+
+  method GetEncryptedDataKeyDescription(config: InternalConfig, input: GetEncryptedDataKeyDescriptionInput)
+    returns (output: Result<GetEncryptedDataKeyDescriptionOutput, Error>)
+    ensures GetEncryptedDataKeyDescriptionEnsuresPublicly(input, output)
+    ensures output.Success? ==> (    
+      match input.input {
+        case plaintextItem(item) => 
+          "aws_dbe_head" in DynamoToStruct.ItemToStructured(item).Extract().Keys
+          && Header.PartialDeserialize(DynamoToStruct.ItemToStructured(item).Extract()["aws_dbe_head"].content.Terminal.value).Success?
+        case header(header) => 
+          Header.PartialDeserialize(header).Success?
+      }
+    )
+  {
+    var header;
+    match input.input
+    {
+      case plaintextItem(plaintextItem) =>{
+        header := DynamoToStruct.ItemToStructured(plaintextItem).Extract()["aws_dbe_head"].content.Terminal.value;
+      }
+      case header(headeritem) => {
+        header := headeritem;
+      } 
+    }
+    var deserializedHeader := Header.PartialDeserialize(header);
+    print deserializedHeader;
+
+    var algorithmSuite;
+    if deserializedHeader.Extract().flavor == 0{
+      algorithmSuite := AlgorithmSuites.DBE_ALG_AES_256_GCM_HKDF_SHA512_COMMIT_KEY_SYMSIG_HMAC_SHA384;
+    }
+    else{
+      algorithmSuite := AlgorithmSuites.DBE_ALG_AES_256_GCM_HKDF_SHA512_COMMIT_KEY_ECDSA_P384_SYMSIG_HMAC_SHA384;
+    }
+
+    var datakeys := deserializedHeader.Extract().dataKeys;
+    var list : EncryptedDataKeyDescriptionList;
+    for i := 0 to |datakeys| {
+      var singleDataKeyOutput : EncryptedDataKeyDescriptionOutput;
+      if UTF8.Decode(datakeys[i].keyProviderId).Extract() == "aws-kms-hierarchy" {
+
+        var providerWrappedMaterial := EdkWrapping.GetProviderWrappedMaterial(datakeys[i].ciphertext, algorithmSuite).Extract();
+
+        var EDK_CIPHERTEXT_BRANCH_KEY_VERSION_INDEX := 12 + 16;
+        var EDK_CIPHERTEXT_VERSION_INDEX := EDK_CIPHERTEXT_BRANCH_KEY_VERSION_INDEX + 16;
+
+        var branchKeyVersionUuid := providerWrappedMaterial[EDK_CIPHERTEXT_BRANCH_KEY_VERSION_INDEX .. EDK_CIPHERTEXT_VERSION_INDEX];
+      
+        singleDataKeyOutput := EncryptedDataKeyDescriptionOutput(
+          keyProviderId := UTF8.Decode(datakeys[i].keyProviderId).Extract(),
+          keyProviderInfo := UTF8.Decode(datakeys[i].keyProviderInfo).Extract(), 
+          branchKeyId := Some(UTF8.Decode(datakeys[i].keyProviderInfo).Extract()),
+          branchKeyVersion := Some(UUID.FromByteArray(branchKeyVersionUuid).Extract())
+        );
+      }
+      else {
+        singleDataKeyOutput := EncryptedDataKeyDescriptionOutput(
+          keyProviderId := UTF8.Decode(datakeys[i].keyProviderId).Extract(),
+          keyProviderInfo := UTF8.Decode(datakeys[i].keyProviderInfo).Extract(), 
+          branchKeyId := None,
+          branchKeyVersion := None
+        );
+      }
+      list := list + [singleDataKeyOutput];
+    }
+  
+    output := Success(GetEncryptedDataKeyDescriptionOutput(
+                        EncryptedDataKeyDescriptionOutput := list
+                      ));
   }
 }
